src/ElimFuncComp2.v
@@ -1403,7 +1403,10 @@ Section Preservation.
   Proof.
     eapply Semantics.forward_simulation_star with (match_states := I' (fst prog) (fst tprog)).
     - admit. (* TODO - replace with callstate matching *)
-    - intros0 II Afinal. invc Afinal. invc II. on >I, invc. constructor. eauto using I_expr_value.
+    - intros0 II Afinal. invc Afinal. invc II. on >I, invc.
+      eexists. split.
+      constructor. eauto using I_expr_value.
+      reflexivity.
     - intros0 Astep. intros0 II.
       eapply sstar_semantics_sim, I'_sim; try eassumption.
       + destruct prog, tprog. eapply compile_cu_compile_list; eauto.
