src/TopLevel.v
@@ -1,0 +1,84 @@
+Require Import MixSemantics.
+
+Require Import StructTact.StructTactics.
+Require Import StructTact.Util.
+
+Require Import EricTact.
+
+Section Spec.
+
+  Variable T1 T2 : Type.
+  Variable p1 : T1.
+  Variable p2 : T2.
+  Variable sem1 : T1 -> notrace_semantics.
+  Variable sem2 : T2 -> trace_semantics.
+  Variable fsim : mix_forward_simulation (sem1 p1) (sem2 p2).
+
+  Definition L1 := sem1 p1.
+  Definition L2 := sem2 p2.
+  Definition ge := Semantics.globalenv L1.
+  Definition tge := TraceSemantics.globalenv L2.
+  Definition step1 := Semantics.step L1.
+  Definition step2 := TraceSemantics.step L2.
+    
+  Definition match_states := (fsim_match_states _ _ fsim).
+  Definition match_values := (fsim_match_val _ _ fsim).
+
+  Lemma establish_matching :
+    forall f v lst hf hv,
+      TraceSemantics.is_callstate (sem2 p2) f v lst -> (* This is what the users need to establish *)
+      match_values hf f -> (* this too *)
+      match_values hv v -> (* this as well *)
+      exists hst i,
+        Semantics.is_callstate (sem1 p1) hf hv hst /\
+        match_states i hst lst.
+  Proof.        
+    intros.
+    unfold match_values in *. unfold MixSemantics.fsim_match_val in *.
+    eapply (MixSemantics.fsim_match_callstate _ _ fsim) in H; eauto.
+    destruct H. destruct H. destruct H.
+    repeat eexists; repeat split; eauto.
+  Qed.
+
+  Lemma star_step_simulation :
+    forall hst hst',
+      Semantics.star _ _ step1 ge hst hst' ->
+      forall i lst,
+        match_states i hst lst ->
+        exists lst' i',
+          TraceSemantics.star step2 tge lst Events.E0 lst' /\
+          match_states i' hst' lst'.
+  Proof.
+    induction 1; intros.
+    repeat eexists. eapply TraceSemantics.star_refl.
+    eassumption.
+    eapply (MixSemantics.fsim_simulation _ _ fsim) in H; eauto.
+    repeat (break_exists || break_and).
+    destruct H. fold match_states in H2.
+    specialize (IHstar _ _ H2).
+    edestruct IHstar. repeat break_exists; break_and.
+    exists x1. exists x2.
+    split. eapply TraceSemantics.star_trans; nil_trace.
+    eapply TraceSemantics.plus_star; eauto.
+    eauto. eauto.
+    specialize (IHstar _ _ H2).
+    repeat break_exists; break_and.
+    exists x1. exists x2.
+    split. eapply TraceSemantics.star_trans; nil_trace.
+    eauto. eauto.
+    eauto.
+  Qed.
+
+  Lemma final_states :
+    forall i hst lst hv,
+      match_states i hst lst ->
+      Semantics.final_state L1 hst hv ->
+      exists lv,
+        TraceSemantics.final_state L2 lst lv /\ match_values hv lv.
+  Proof.
+    intros.
+    eapply (MixSemantics.fsim_match_final_states) in H0; eauto.
+  Qed.
+
+  
+End Spec.
